Rough outline of semantics reflection proof for trans_alt

projection/proofs/payload_closureProofScript.sml
@@ -1,5 +1,5 @@
 open preamble payloadSemTheory payloadLangTheory choreoUtilsTheory payload_closureTheory payloadPropsTheory
-     payload_bisimTheory payloadConfluenceTheory ConseqConv;
+     payload_bisimTheory payloadConfluenceTheory ConseqConv payload_altSemTheory payload_altPropsTheory;
 
 val _ = new_theory "payload_closureProof";
 
@@ -580,10 +580,22 @@ Definition compile_rel_def:
   )
 End
 
+Definition compile_rel_alt_def:
+  compile_rel_alt conf n1 n2 =
+  (letrec_network n1 ∧ letrec_network n2 ∧
+   BISIM_REL (trans_alt conf) n1 n2)
+End
+
 Theorem compile_rel_refl:
   letrec_network x ⇒ compile_rel conf x x
 Proof
   rw[compile_rel_def,tausim_refl]
+QED
+
+Theorem compile_rel_alt_refl:
+  letrec_network x ⇒ compile_rel_alt conf x x
+Proof
+  metis_tac[compile_rel_alt_def,bisimulationTheory.BISIM_REL_IS_EQUIV_REL,equivalence_def,reflexive_def]
 QED
 
 Theorem compile_rel_reflI:
@@ -956,14 +968,6 @@ Proof
   fs[]
 QED
 
-Theorem ALOOKUP_ZIP_SELF:
-  ALOOKUP (ZIP (l,l)) x =
-  if MEM x l then SOME x else NONE
-Proof
-  Induct_on ‘l’ >>
-  rw[] >> fs[]
-QED
-
 Theorem ALOOKUP_REVERSE_ALL_DISTINCT:
   ALL_DISTINCT (MAP FST l) ⇒
   ALOOKUP (REVERSE l) = ALOOKUP l
@@ -1242,12 +1246,6 @@ Proof
        fs[] >> rveq >>
        goal_assum(resolve_then (Pos hd) mp_tac RC_SUBSET) >>
        simp[reduction_def,Once trans_cases])
-QED
-
-Triviality RC_REFL:
-  RC R x x
-Proof
-  rw[RC_DEF]
 QED
 
 Theorem tausim_defer_fundef:
@@ -3531,6 +3529,13 @@ Proof
   rw[compile_rel_def] >> metis_tac[tausim_trans]
 QED
 
+Theorem compile_rel_alt_trans:
+  compile_rel_alt conf p1 p2 ∧ compile_rel_alt conf p2 p3 ⇒
+  compile_rel_alt conf p1 p3
+Proof
+  rw[compile_rel_alt_def] >> metis_tac[bisimulationTheory.BISIM_REL_IS_EQUIV_REL,equivalence_def,transitive_def]
+QED
+
 (* TODO: having compile_network instead of compile_network_alt in the conclusion would be
          nicer, but that requires using a different notion of bismulation in the theorem statement *)
 Theorem compile_network_preservation_trans:
@@ -3553,25 +3558,237 @@ Proof
     simp[compile_rel_def,letrec_network_compile_network,letrec_network_compile_network_alt] *)
 QED
 
-(*
-Theorem compile_network_preservation:
-  ∀conf p1 p2.
-    conf.payload_size > 0
-    ∧ reduction^* p1 p2 ∧ choice_free_network p1
-    ==> (reduction conf)^* (compile_network conf p1) (compile_network conf p2)
+Theorem tausim_reductionE:
+  ∀conf p2 p3 p1.
+  (reduction conf)^* p2 p3 ∧
+  tausim conf p1 p2 ⇒
+  ∃p4. (reduction conf)^* p1 p4 ∧ tausim conf p4 p3
 Proof
-  strip_tac >> simp[GSYM AND_IMP_INTRO,RIGHT_FORALL_IMP_THM]
-  >> strip_tac
-  >> ho_match_mp_tac RTC_INDUCT
-  >> rpt strip_tac
-  >- simp[]
-  >> fs[reduction_def]
-  >> imp_res_tac choice_free_trans_pres
-  >> first_x_assum drule >> strip_tac
-  >> fs[GSYM reduction_def]
-  >> drule compile_network_preservation_trans >> simp[Once CONJ_SYM]
-  >> rpt(disch_then drule) >> strip_tac >> metis_tac[RTC_RTC]
+  strip_tac >>
+  simp[GSYM PULL_FORALL,GSYM AND_IMP_INTRO] >>
+  ho_match_mp_tac RTC_STRONG_INDUCT >> rw[]
+  >- metis_tac[RTC_REFL,tausim_refl]
+  >- (qhdtm_x_assum ‘tausim’ (strip_assume_tac o REWRITE_RULE[Once tausim_cases]) >>
+      fs[reduction_def] >>
+      res_tac >> fs[] >>
+      last_x_assum drule >> rw[] >>
+      goal_assum(drule_at (Pos last)) >>
+      drule_at_then (Pos last) match_mp_tac RTC_RTC >>
+      drule_then MATCH_ACCEPT_TAC RC_RTC)
 QED
-*)
+
+Theorem tausim_reductionE2:
+  ∀conf p2 p3 p1.
+  reduction conf p1 p3 ∧
+  tausim conf p1 p2 ⇒
+  ∃p4. (reduction conf)^+ p2 p4 ∧ tausim conf p3 p4
+Proof
+  strip_tac >>
+  rw[Once tausim_cases,reduction_def]
+QED
+
+Theorem compile_network_preservation_alt:
+  ∀conf p1 p2.
+    (reduction conf)^* p1 p2
+    ∧ conf.payload_size > 0
+    ∧ fix_network p1
+    ∧ free_fix_names_network p1 = []
+    ∧ no_undefined_vars_network p1
+    ⇒ ∃p3. (reduction conf)^* (compile_network_alt p1) p3 ∧
+           compile_rel conf p3 (compile_network_alt p2)
+Proof
+  strip_tac >>
+  simp[GSYM AND_IMP_INTRO] >>
+  ho_match_mp_tac RTC_STRONG_INDUCT >>
+  rw[] >-
+    (goal_assum(resolve_then (Pos hd) mp_tac RTC_REFL) >>
+     match_mp_tac compile_rel_refl >>
+     simp[letrec_network_compile_network_alt]) >>
+  fs[] >>
+  ‘fix_network p1'’ by metis_tac[fix_network_trans_pres,reduction_def] >>
+  first_x_assum drule >>
+  impl_tac >- cheat >>
+  strip_tac >>
+  drule_all compile_network_preservation_trans_alt >>
+  strip_tac >>
+  qhdtm_assum ‘compile_rel’ (strip_assume_tac o REWRITE_RULE[compile_rel_def]) >>
+  drule_all tausim_reductionE >>
+  strip_tac >>
+  goal_assum(resolve_then (Pos hd) mp_tac RTC_RTC) >>
+  goal_assum drule >>
+  goal_assum drule >>
+  fs[compile_rel_def] >>
+  conj_tac >- cheat >>
+  metis_tac[tausim_trans]
+QED
+
+Theorem compile_network_reflection_alt_single:
+  ∀p1 p2 conf.
+    conf.payload_size > 0
+    ∧ fix_network p1
+    ∧ free_fix_names_network p1 = []
+    ∧ no_undefined_vars_network p1
+    ∧ (reduction_alt conf) (compile_network_alt p1) p2
+    ⇒ ∃p3 p4. reduction_alt conf p1 p3 ∧
+              (reduction_alt conf)^* p2 p4 ∧
+              compile_rel_alt conf p4 (compile_network_alt p3)
+Proof
+  cheat
+QED
+
+Theorem compile_network_alt_endpoints:
+  ∀p1.
+    MAP FST(endpoints(compile_network_alt p1)) = MAP FST (endpoints p1)
+Proof
+  Induct >> rw[compile_network_alt_def,endpoints_def]
+QED
+
+Theorem compile_network_endpoints:
+  ∀p1.
+    MAP FST(endpoints(compile_network p1)) = MAP FST (endpoints p1)
+Proof
+  Induct >> rw[compile_network_def,endpoints_def]
+QED
+
+Theorem letrec_network_trans_alt_pres:
+  letrec_network p1 ∧ trans_alt conf p1 α p2 ⇒ letrec_network p2
+Proof
+  rw[] >> Cases_on ‘α ≠ LTau’ >>
+  fs[trans_alt_nontau_eq,GSYM reduction_alt_def] >>
+  imp_res_tac letrec_network_trans_pres >>
+  drule reduction_alt_IMP >>
+  qhdtm_x_assum ‘letrec_network’ mp_tac >>
+  simp[AND_IMP_INTRO] >>
+  match_mp_tac RTC_lifts_invariants >>
+  metis_tac[letrec_network_trans_pres,reduction_def]
+QED
+
+Theorem fix_network_trans_alt_pres:
+  fix_network p1 ∧ trans_alt conf p1 α p2 ⇒ fix_network p2
+Proof
+  rw[] >> Cases_on ‘α ≠ LTau’ >>
+  fs[trans_alt_nontau_eq,GSYM reduction_alt_def] >>
+  imp_res_tac fix_network_trans_pres >>
+  drule reduction_alt_IMP >>
+  qhdtm_x_assum ‘fix_network’ mp_tac >>
+  simp[AND_IMP_INTRO] >>
+  match_mp_tac RTC_lifts_invariants >>
+  metis_tac[fix_network_trans_pres,reduction_def]
+QED
+
+Theorem compile_rel_alt_trans_alt_pres:
+ ∀conf p1 p2 l p3.
+ compile_rel_alt conf p1 p2 ∧
+ trans_alt conf p1 l p3 ⇒
+ ∃p4. trans_alt conf p2 l p4 ∧ compile_rel_alt conf p3 p4
+Proof
+  rpt strip_tac >>
+  fs[compile_rel_alt_def] >>
+  qhdtm_x_assum ‘BISIM_REL’ (strip_assume_tac o REWRITE_RULE[Once bisimulationTheory.BISIM_REL_cases]) >>
+  fs[FORALL_AND_THM] >>
+  res_tac >>
+  goal_assum drule >> simp[] >>
+  imp_res_tac letrec_network_trans_alt_pres >> simp[]
+QED
+
+Theorem compile_rel_alt_trans_alt_pres':
+ ∀conf p1 p2 l p3.
+ compile_rel_alt conf p1 p2 ∧
+ trans_alt conf p2 l p3 ⇒
+ ∃p4. trans_alt conf p1 l p4 ∧ compile_rel_alt conf p4 p3
+Proof
+  rpt strip_tac >>
+  fs[compile_rel_alt_def] >>
+  qhdtm_x_assum ‘BISIM_REL’ (strip_assume_tac o REWRITE_RULE[Once bisimulationTheory.BISIM_REL_cases]) >>
+  fs[FORALL_AND_THM] >>
+  res_tac >>
+  goal_assum drule >> simp[] >>
+  imp_res_tac letrec_network_trans_alt_pres >> simp[]
+QED
+
+Theorem compile_rel_alt_list_trans:
+ ∀conf p1 p2 l p3.
+ compile_rel_alt conf p1 p2 ∧
+ list_trans_alt conf p1 l p3 ⇒
+ ∃p4. list_trans_alt conf p2 l p4 ∧ compile_rel_alt conf p3 p4
+Proof
+  strip_tac >>
+  Induct_on ‘l’ >>
+  rw[list_trans_alt_def] >> rw[] >>
+  imp_res_tac compile_rel_alt_trans_alt_pres >>
+  res_tac >>
+  metis_tac[]
+QED
+
+Theorem compile_rel_alt_list_trans':
+ ∀conf p1 p2 l p3.
+ compile_rel_alt conf p1 p2 ∧
+ list_trans_alt conf p2 l p3 ⇒
+ ∃p4. list_trans_alt conf p1 l p4 ∧ compile_rel_alt conf p4 p3
+Proof
+  strip_tac >>
+  Induct_on ‘l’ >>
+  rw[list_trans_alt_def] >> rw[] >>
+  imp_res_tac compile_rel_alt_trans_alt_pres' >>
+  res_tac >>
+  metis_tac[]
+QED
+
+Theorem compile_network_reflection_al_trans_altt:
+  ∀p1 p2 conf.
+    conf.payload_size > 0
+    ∧ fix_network p1
+    ∧ free_fix_names_network p1 = []
+    ∧ no_undefined_vars_network p1
+    ∧ ALL_DISTINCT (MAP FST (endpoints p1))
+    ∧ (reduction_alt conf)^* (compile_network_alt p1) p2
+    ⇒ ∃p3 p4. (reduction_alt conf)^* p1 p3 ∧
+              (reduction_alt conf)^* p2 p4 ∧
+              compile_rel_alt conf p4 (compile_network_alt p3)
+Proof
+  simp[reduction_list_trans_alt,PULL_EXISTS] >>
+  CONV_TAC(RESORT_FORALL_CONV rev) >>
+  ho_match_mp_tac COMPLETE_INDUCTION >>
+  Cases
+  >- (rw[list_trans_alt_def] >>
+      CONV_TAC(RESORT_EXISTS_CONV rev) >>
+      qexists_tac `0` >> qexists_tac ‘0’ >> rw[list_trans_alt_def] >>
+      metis_tac[RTC_REFL,compile_rel_alt_refl,letrec_network_compile_network_alt])
+  >- (rw[list_trans_alt_def,GSYM reduction_alt_def] >>
+      drule_all(compile_network_reflection_alt_single
+                |> REWRITE_RULE[PULL_EXISTS,reduction_list_trans]) >>
+      strip_tac >>
+      fs[reduction_list_trans_alt] >>
+      dxrule payload_confluence_weak_contract_alt >>
+      disch_then drule >>
+      impl_tac
+      >- (metis_tac[endpoint_names_trans_alt,reduction_alt_def,
+                    compile_network_alt_endpoints]) >>
+      strip_tac >>
+      drule_all compile_rel_alt_list_trans >>
+      strip_tac >>
+      rename1 `list_trans_alt _ (compile_network_alt _) (REPLICATE stepcount _) _` >>
+      first_x_assum(qspec_then `stepcount` mp_tac ) >>
+      impl_tac >- simp[] >>
+      disch_then drule >>
+      fs[reduction_alt_def] >>
+      drule_all_then strip_assume_tac fix_network_trans_alt_pres >>
+      disch_then drule >>
+      disch_then(drule_at (Pos last)) >>
+      impl_tac >- cheat >>
+      strip_tac >>
+      CONV_TAC(RESORT_EXISTS_CONV rev) >>
+      CONV_TAC SWAP_EXISTS_CONV >>
+      Q.REFINE_EXISTS_TAC ‘SUC _’ >>
+      simp[list_trans_alt_def,PULL_EXISTS] >>
+      goal_assum drule >>
+      goal_assum drule >>
+      drule_all compile_rel_alt_list_trans' >>
+      strip_tac >>
+      Q.REFINE_EXISTS_TAC ‘_ + _’ >>
+      simp[GSYM REPLICATE_APPEND,list_trans_alt_append,PULL_EXISTS] >>
+      rpt(goal_assum drule) >>
+      metis_tac[compile_rel_alt_trans])
+QED
 
 val _ = export_theory ();
